## Derivada de Funciones
| Función | Derivada |
|---------|----------|
| <span style="font-size: 1.5em;">$f(x) = c$</span> (constante) | <span style="font-size: 1.5em;">$f'(x) = 0$</span> |
| <span style="font-size: 1.5em;">$f(x) = x^n$</span> | <span style="font-size: 1.5em;">$f'(x) = nx^{n-1}$</span> |
| <span style="font-size: 1.5em;">$f(x) = e^x$</span> | <span style="font-size: 1.5em;">$f'(x) = e^x$</span> |
| <span style="font-size: 1.5em;">$f(x) = a^x$</span> | <span style="font-size: 1.5em;">$f'(x) = a^x \ln(a)$</span> |
| <span style="font-size: 1.5em;">$f(x) = \ln(x)$</span> | <span style="font-size: 1.5em;">$f'(x) = \frac{1}{x}$</span> |
| <span style="font-size: 1.5em;">$f(x) = \log_a(x)$</span> | <span style="font-size: 1.5em;">$f'(x) = \frac{1}{x \ln(a)}$</span> |
| <span style="font-size: 1.5em;">$f(x) = \sin(x)$</span> | <span style="font-size: 1.5em;">$f'(x) = \cos(x)$</span> |
| <span style="font-size: 1.5em;">$f(x) = \cos(x)$</span> | <span style="font-size: 1.5em;">$f'(x) = -\sin(x)$</span> |
| <span style="font-size: 1.5em;">$f(x) = \tan(x)$</span> | <span style="font-size: 1.5em;">$f'(x) = \sec^2(x)$</span> |
| <span style="font-size: 1.5em;">$f(x) = \cot(x)$</span> | <span style="font-size: 1.5em;">$f'(x) = -\csc^2(x)$</span> |
| <span style="font-size: 1.5em;">$f(x) = \sec(x)$</span> | <span style="font-size: 1.5em;">$f'(x) = \sec(x)\tan(x)$</span> |
| <span style="font-size: 1.5em;">$f(x) = \csc(x)$</span> | <span style="font-size: 1.5em;">$f'(x) = -\csc(x)\cot(x)$</span> |
| <span style="font-size: 1.5em;">$f(x) = \arcsin(x)$</span> | <span style="font-size: 1.5em;">$f'(x) = \frac{1}{\sqrt{1-x^2}}$</span> |
| <span style="font-size: 1.5em;">$f(x) = \arccos(x)$</span> | <span style="font-size: 1.5em;">$f'(x) = -\frac{1}{\sqrt{1-x^2}}$</span> |
| <span style="font-size: 1.5em;">$f(x) = \arctan(x)$</span> | <span style="font-size: 1.5em;">$f'(x) = \frac{1}{1+x^2}$</span> |
| <span style="font-size: 1.5em;">$f(x) = \sinh(x)$</span> | <span style="font-size: 1.5em;">$f'(x) = \cosh(x)$</span> |
| <span style="font-size: 1.5em;">$f(x) = \cosh(x)$</span> | <span style="font-size: 1.5em;">$f'(x) = \sinh(x)$</span> |
| <span style="font-size: 1.5em;">$f(x) = \tanh(x)$</span> | <span style="font-size: 1.5em;">$f'(x) = \text{sech}^2(x)$</span> |

## Reglas de derivación

| Regla | Derivada |
|-------|----------|
| Suma: <span style="font-size: 1.5em;">$f(x) = g(x) + h(x)$</span> | <span style="font-size: 1.5em;">$f'(x) = g'(x) + h'(x)$</span> |
| Resta: <span style="font-size: 1.5em;">$f(x) = g(x) - h(x)$</span> | <span style="font-size: 1.5em;">$f'(x) = g'(x) - h'(x)$</span> |
| Producto: <span style="font-size: 1.5em;">$f(x) = g(x)h(x)$</span> | <span style="font-size: 1.5em;">$f'(x) = g'(x)h(x) + g(x)h'(x)$</span> |
| Cociente: <span style="font-size: 1.5em;">$f(x) = \frac{g(x)}{h(x)}$</span> | <span style="font-size: 1.5em;">$f'(x) = \frac{g'(x)h(x) - g(x)h'(x)}{[h(x)]^2}$</span> |
| Cadena: <span style="font-size: 1.5em;">$f(x) = g(h(x))$</span> | <span style="font-size: 1.5em;">$f'(x) = g'(h(x)) \cdot h'(x)$</span> |
| Potencia: <span style="font-size: 1.5em;">$f(x) = [g(x)]^n$</span> | <span style="font-size: 1.5em;">$f'(x) = n[g(x)]^{n-1} \cdot g'(x)$</span> |
| Exponencial: <span style="font-size: 1.5em;">$f(x) = e^{g(x)}$</span> | <span style="font-size: 1.5em;">$f'(x) = e^{g(x)} \cdot g'(x)$</span> |
| Logarítmica: <span style="font-size: 1.5em;">$f(x) = \ln(g(x))$</span> | <span style="font-size: 1.5em;">$f'(x) = \frac{g'(x)}{g(x)}$</span> |


## Derivadas de funciones inversas

| Función | Derivada |
|---------|----------|
| <span style="font-size: 1.5em;">$f(x) = g^{-1}(x)$</span> | <span style="font-size: 1.5em;">$f'(x) = \frac{1}{g'(g^{-1}(x))}$</span> |

